

Group Members:

- Nabil Arrouss (qup85ses)
- Ahmad Pamir Sahak (las06weq)
- Kohei Fujimura (koj66veq)
- Heydar Bagloo (yeq42hip)

Exercise 1:

$$P(H|E_1=e_1, E_2=e_2) \text{ for } H \in \{1, \dots, k\}$$

$$P(H|e_1, e_2) = \frac{P(H, e_1, e_2)}{P(e_1, e_2)} = \frac{P(H) P(e_1, e_2|H)}{P(e_1, e_2)}$$

ii) $P(e_1, e_2), P(H), P(e_1, e_2|H)$, $P(H, e_1, e_2) = P(H) P(e_1, e_2|H)$

$$\Rightarrow P(H|e_1, e_2) = \frac{P(H) P(e_1, e_2|H)}{P(e_1, e_2)}$$

$$\Rightarrow P(e_1, e_2) = \sum_{H=1}^k P(H) P(e_1, e_2|H)$$

iv) $P(H|e_1, e_2) = \frac{P(H, e_1, e_2)}{P(e_1, e_2)}$

$$\Rightarrow P(e_1, e_2) = \sum_{H=1}^k P(H, e_1, e_2)$$

$$\Rightarrow P(H|e_1, e_2) = \frac{P(H, e_1, e_2)}{\sum_{H=1}^k P(H, e_1, e_2)}$$

ii and iv are sufficient.

b) $E_1 \perp E_2 | H$ (conditional independence)

$$P(e_1, e_2|H) = P(e_1|H) P(e_2|H)$$

$$\Rightarrow P(H|e_1, e_2) = \frac{P(H) P(e_1|H) \cdot P(e_2|H)}{P(e_1, e_2)}, \quad P(e_1, e_2) = \sum_H P(H) P(e_1|H) P(e_2|H)$$

i) we can form the numerator $P(H) \cdot P(e_1|H) \cdot P(e_2|H)$ and the denominator is given so we can compute the posterior.

- Sufficient under the independence assumption.

ii) sufficient without independence.

iii) Using conditional independence we can compute

$P(e_1, e_2) = \sum_H P(H) P(e_1|H) P(e_2|H)$ so we can compute numerator and denominator and posterior.

- Sufficient under the independence assumption

iv; Sufficien (we know from part a)

Exercise 2:

a) $X_1, X_2, X_3 \in \{0, 1\}$, X_1, X_2 are independent fair coin

$$P(X_1=0) = P(X_1=1) = \frac{1}{2}, \quad P(X_2=0) = P(X_2=1) = \frac{1}{2}, \quad X_1 \perp X_2$$

$$X_3 = X_1 \oplus X_2 \Rightarrow X_3=0, \text{ if } X_1 \text{ and } X_2 \text{ are equal, } X_3=1, \text{ if } X_1 \neq X_2$$

$$\text{each } X_i \quad P(X_i=0) = P(X_i=1) = \frac{1}{2}$$

X_1 and X_3 for example:

$$P(X_1=0, X_3=0) = P(0,0,0) = \frac{1}{4}$$

$$\Rightarrow P(X_1=0) P(X_3=0) = \frac{1}{2} \cdot \frac{1}{2} = \frac{1}{4}$$

But

$$P(X_1=0, X_2=0, X_3=0) = \frac{1}{4}$$

$$P(X_1=0) P(X_2=0) P(X_3=0) = \frac{1}{2} \cdot \frac{1}{2} \cdot \frac{1}{2} = \frac{1}{8}$$

Since $\frac{1}{4} \neq \frac{1}{8}$ so $P(X_1, X_2, X_3) \neq P(X_1) \cdot P(X_2) \cdot P(X_3)$

b)

assume that X_1, \dots, X_n are mutually independent by:

$$P(X_1=x_1, \dots, X_n=x_n) = \prod_{i=1}^n P(X_i=x_i)$$

$$\Rightarrow P(X_i=x_i, X_j=x_j) = \sum_{\substack{X_k \in \{0,1\} \\ k \neq i,j}} P(X_1=x_1, \dots, X_n=x_n) = \sum_{\substack{X_k \in \{0,1\} \\ k \neq i,j}} \prod_{m=1}^n P(X_m=x_m)$$

Since

$$P(X_i=x_i, X_j=x_j) = (P(X_i=x_i) P(X_j=x_j)) \cdot \prod_{\substack{k \neq i,j}} \left(\sum_{X_k} P(X_k=x_k) \right)$$

$$\text{and } \forall k, \sum_{X_k} P(X_k=x_k) = 1$$

$$\text{so } P(X_i=x_i, X_j=x_j) = P(X_i=x_i) P(X_j=x_j)$$

$$c) P(X_1|X_2) = P(X_1)$$

, suppose X_1, X_2 independent

$$P(X_1=x_1, X_2=x_2) = P(X_1=x_1) P(X_2=x_2)$$

for all x_1, x_2 , if $P(X_2=x_2) > 0$ then:

$$P(X_1=x_1 | X_2=x_2) = \frac{P(X_1=x_1, X_2=x_2)}{P(X_2=x_2)} = \frac{P(X_1=x_1) \cdot P(X_2=x_2)}{P(X_2=x_2)}$$

$$\Rightarrow P(X_1=x_1)$$

Exercise 3:

$$\text{Bias}[\hat{\theta}] = E[\hat{\theta}] - \theta^*$$

$$\text{Var}[\hat{\theta}] = E[(\hat{\theta} - E[\hat{\theta}])^2]$$

$$\text{MSE} = E[(\hat{\theta} - \theta^*)^2]$$

$$\Rightarrow E[(\hat{\theta} - \theta^*)^2] \quad , \quad \hat{\theta} - \theta^* = (\hat{\theta} - E[\hat{\theta}]) + (E[\hat{\theta}] - \theta^*)$$

$$\Rightarrow (\hat{\theta} - \theta^*)^2 = [(\hat{\theta} - E[\hat{\theta}]) + (E[\hat{\theta}] - \theta^*)]^2$$

$$\Rightarrow (\hat{\theta} - E[\hat{\theta}])^2 + 2(\hat{\theta} - E[\hat{\theta}])(E[\hat{\theta}] - \theta^*) + (E[\hat{\theta}] - \theta^*)^2$$

$$\Rightarrow E[(\hat{\theta} - \theta^*)^2] = E[(\hat{\theta} - E[\hat{\theta}])^2] + 2E[(\hat{\theta} - E[\hat{\theta}])(E[\hat{\theta}] - \theta^*)] + E[(E[\hat{\theta}] - \theta^*)^2]$$

$$E[(\hat{\theta} - E[\hat{\theta}])^2] = \text{Var}[\hat{\theta}]$$

$$2(E[\hat{\theta}] - \theta^*)E[\hat{\theta} - E[\hat{\theta}]] \quad , \quad E[\hat{\theta} - E[\hat{\theta}]] = 0$$

$$E[(E[\hat{\theta}] - \theta^*)^2] = (E[\hat{\theta} - \theta^*])^2 = (\text{Bias}[\hat{\theta}])^2$$

$$\Rightarrow E[(\hat{\theta} - \theta^*)^2] = \text{Var}[\hat{\theta}] + (\text{Bias}[\hat{\theta}])^2$$

$$\Rightarrow \text{MSE}[\hat{\theta}] = \text{Var}[\hat{\theta}] + (\text{Bias}[\hat{\theta}])^2$$

Ex 4:
a)

$$l = \ln L = \ln \left(\prod_{i=1}^N \mathcal{N}(x_i | \mu, \sigma^2) \right)$$

$$\ln \left(\prod_{i=1}^N \frac{1}{\sigma \sqrt{2\pi}} \cdot e^{-\frac{1}{2} \left(\frac{x_i - \mu}{\sigma} \right)^2} \right)$$

$$= \sum_{i=1}^N \ln \left(\frac{1}{\sigma \sqrt{2\pi}} \cdot e^{-\frac{1}{2} \left(\frac{x_i - \mu}{\sigma} \right)^2} \right)$$

$$= \sum_{i=1}^N \ln \left(\frac{1}{\sigma \sqrt{2\pi}} \right) - \frac{1}{2} \sum_{i=1}^N \left(\frac{x_i - \mu}{\sigma} \right)^2$$

$$= \ln \left(\frac{1}{\sigma \sqrt{2\pi}} \right) - \frac{1}{2} \sum_{i=1}^N \left(\frac{x_i - \mu}{\sigma} \right)^2$$

$$b) \frac{\partial l}{\partial \mu} = \frac{\partial l}{\partial \mu} \left(-\frac{1}{2\sigma^2} \sum_{i=1}^N (x_i - \mu)^2 \right)$$

$$= -\frac{1}{2\sigma^2} \left(\sum_{i=1}^N -2(x_i - \mu) \right)$$

$$= \frac{1}{\sigma^2} \sum_{i=1}^N (x_i - \mu) \stackrel{!}{=} 0$$

$$= \frac{1}{\sigma^2} \sum_{i=1}^N x_i - \sum_{i=1}^N \mu$$

$$= \frac{1}{\sigma^2} \sum_{i=1}^N x_i - N\mu = 0$$

The term is 0 if $\sum_{i=1}^N x_i - N\mu = 0$

$$\sum_{i=1}^N x_i - N\mu \stackrel{!}{=} 0$$

$$\sum_{i=1}^N x_i = N\mu \Rightarrow \hat{\mu} = \frac{1}{N} \sum_{i=1}^N x_i$$

$$d) \text{bias}[\hat{\mu}] = E[\hat{\mu} - \mu^*]$$

$$= E\left[\frac{1}{N} \sum_{i=1}^N x_i - \mu^*\right]$$

$$= E\left[\frac{1}{N} \sum_{i=1}^N x_i\right] - E[\mu^*]$$

$$= \frac{1}{N} E\left[\sum_{i=1}^N x_i\right] - E[\mu^*]$$

$$= \frac{1}{N} \sum_{i=1}^N E[x_i] - E[\mu^*]$$

$$= \frac{1}{N} \sum_{i=1}^N \mu^* - \mu^* = 0$$

$$e) \text{var}[\hat{\mu}] = \text{var}\left[\frac{1}{N} \sum_{i=1}^N x_i\right]$$

$$= \frac{1}{N^2} \sum_{i=1}^N \text{var}[x_i]$$

$$f) \text{mse}[\hat{\mu}] = \text{bias}[\hat{\mu}]^2 + \text{var}[\hat{\mu}]$$

$$= \left(\frac{1}{N} \sum_{i=1}^N E[x_i] - E[\mu^*]\right)^2 + \frac{1}{N^2} \sum_{i=1}^N \text{var}[x_i]$$

$$= \frac{1}{N^2} \sum_{i=1}^N E[x_i]^2 - 2 \cdot \frac{1}{N} \sum_{i=1}^N E[x_i] E[\mu^*] + E[\mu^*]^2 + \frac{1}{N^2} \sum_{i=1}^N \text{var}[x_i]$$

$$= \frac{1}{N^2} \left[\sum_{i=1}^N E[x_i] + \sum_{i=1}^N \text{var}[x_i] \right] - \frac{2}{N} \sum_{i=1}^N E[x_i] E[\mu^*]$$

Machine Learning - Exercise sheet 1

Exercise 5) $D = \{x_1, \dots, x_N\}$ & $p(x|\lambda) = \lambda e^{-\lambda x}$

$x \geq 0$
 $\lambda > 0$

Likelihood:

$$L(\lambda) = \prod_{i=1}^N \lambda e^{-\lambda x_i} = \lambda^N \exp\left(-\lambda \sum_{i=1}^N x_i\right)$$

Log-likelihood:

$$\ell(\lambda) = \log L(\lambda) = N \log \lambda - \lambda \sum_{i=1}^N x_i$$

$$\frac{d\ell}{d\lambda} = \frac{N}{\lambda} - \sum_{i=1}^N x_i$$

$$\frac{d\ell}{d\lambda} = 0 \Rightarrow \frac{N}{\lambda} - \sum_{i=1}^N x_i = 0$$

$$\Rightarrow \hat{\lambda}_{MLE} = \frac{N}{\sum_{i=1}^N x_i} = \frac{1}{\bar{x}}$$

s.t. \bar{x} is the sample mean.